\documentclass[11pt, oneside]{article} 
\usepackage{geometry}
\geometry{letterpaper} 
\usepackage{graphicx}
	
\usepackage{amssymb}
\usepackage{amsmath}
\usepackage{parskip}
\usepackage{color}
\usepackage{hyperref}

\graphicspath{{/Users/telliott/Dropbox/Github-math/figures/}}
% \begin{center} \includegraphics [scale=0.4] {gauss3.png} \end{center}

\title{Two last proofs of the Pythagorean theorem}
\date{}

\begin{document}
\maketitle
\Large

%[my-super-duper-separator]

\subsection*{Condit proof}

\label{sec:Condit}

Here is a proof by a student named Ann Condit, who was a sophomore in high school at the time.  It is one that Euclid would approve of.

We start by drawing the right $\triangle ABC$ and the squares on each side, as with Euclid $I.47$.

\begin{center} \includegraphics [scale=0.35] {Condit1.png} \end{center}

Next, join two nearby points on the two smaller squares to form $DF$ as shown.  

(1) $\triangle CDF$ is congruent to the original triangle $ABC$, by SAS.

We number our conclusions to keep track of everything, because the proof is a bit longer than many.

Next, find the midpoints of each side of $\triangle ABC$ at $P$, $Q$ and $R$.  

\begin{center} \includegraphics [scale=0.35] {Condit2.png} \end{center}

The line segment joining the midpoints of opposite sides forms a smaller triangle similar to the larger one.  $\triangle BPR$ and $\triangle APQ$ are both similar to $\triangle ABC$ and congruent to each other.  Therefore

(2) $PQ$ and $PR$ form right angles with the sides $AC$ and $CB$, respectively.

(3)  Thus, $CRPQ$ is a rectangle (four right angles), so opposing sides are equal.

We will erase the dotted lines to reduce clutter, but remember the essential property that $P$, $Q$ and $R$ are midpoints;  as well as that $QP$ and $CR$ are parallel sides of a rectangle and equal in length.

We will show that the area of $\triangle APG$ is the sum of the area of $\triangle DQC$ plus that of $\triangle FRC$.  

\begin{center} \includegraphics [scale=0.35] {Condit2b.png} \end{center}

Since each triangle is one-fourth the area of its respective square, this proves that the sum the two smaller squares is equal in area to the largest square.  This is the theorem of Pythagoras.

We need one more line segment.

\begin{center} \includegraphics [scale=0.35] {Condit3.png} \end{center}

Draw $PC$ and extend it to the opposite side $DF$ ending at $E$.  

\subsection*{main idea of the proof}

We claim that $PC$ extended to $CE$, is perpendicular to $DF$.

Recall that when the side of the hypotenuse is bisected in a right triangle, as we did by drawing $CP$, the two resulting smaller triangles are both isosceles.  

(4) Because of this, $\angle ACP$ is equal to the angle at the vertex $A$ ($\angle CAB$) of the original $\triangle ABC$.  $\angle ACP$ is also equal to $\angle EDC$, by congruent triangles. 

(5) $\angle PCB$ is equal to the angle at vertex $B$ ($\angle CBA$) as well as to $\angle EFC$, for the same reason. 

\begin{center} \includegraphics [scale=0.35] {Condit3b.png} \end{center}

(6) Therefore $\triangle CDE$ is similar to $\triangle CEF$, which means that the angles at $E$ are identical and so are right angles.

This is the key step of the proof.  Now we just look at the areas of different triangles.

\begin{center} \includegraphics [scale=0.35] {Condit4.png} \end{center}

First, the area of $\triangle FRC$ (one-quarter of the square of $BC$) is equal to the area of $\triangle FCP$, because they share the base $CF$, and $QP$ is parallel to $CR$ and equal in length to it (opposite sides of a rectangle).

But the area of $\triangle FCP$ is equal to $PC \cdot EF$, because $EF$ is the altitude of $\triangle FCP$ (since $\angle FEP$ is a right angle).

By symmetry, the one-quarter of the small square's area is equal to that of $PC \cdot DE$, so together they equal 
\[ PC \cdot DE + PC \cdot EF = PC \cdot DF \]

But we have that $AP = CP$ and $AG = AB = DF$, so they have the same base and the same height and therefore the same area.  

Thus, the two triangles together have the same area as the triangle with base $AG$ and height $AP$.

$\square$

\subsection*{yet another proof}

Recently (April, 2023) I came across an article by Keith McNulty, referenced on Hacker News.  It's an analysis of a very recent proof of the Pythagorean theorem by two teenagers from New Orleans named Calcea Johnson and Ne'Kiya Jackson.

\url{https://keith-mcnulty.medium.com/heres-how-two-new-orleans-teenagers-found-a-new-proof-of-the-pythagorean-theorem-b4f6e7e9ea2d}

I don't have a reference to an original publication, the article simply refers to a presentation at a meeting.  

McNulty claims that the proof involves trigonometry and that this is novel --- ``[it] might make a few established mathematicians eat their words...because their proof uses trigonometry."

Trigonometry contains two sorts of theorems, those which explicitly depend on the Pythagorean theorem, and those which do not, including some which use similar triangles.  (We hedge the statement because of  the complication that similar triangles can be used to prove the theorem).

The law of cosines is an example of a theorem that depends on Pythagoras, while the law of sines does not.  Naturally, one could not use anything which depends on the Pythagorean theorem to prove the theorem, that would be circular logic.

What this proof mainly does is to use similar triangles, plus the law of sines.  Therefore I think McNulty's claim is wrong. 

 It's still worth taking a look.  The really novel part is the use of infinite series.  We're going to use a geometric series:
 
\[ S = 1 + r + r^2 + \dots + r^n + r^{n+1} + \dots \]
The sum of the first $n$ terms of such a series is
\[ S_n = 1 + r + r^2 + \dots + r^n \]
Provided $|r| < 1$, as $n$ gets large, the terms beyond $r^n$ become negligible, so $S_n$ gets closer and closer to the true sum, $S$.  Now,
\[ (1 - r) \cdot S_n = 1 - r^{n+1} \]
a classic "telescoping" series, and if $r^{n+1}$ and subsequent terms are small enough then
\[ S \approx S_n \approx \frac{1}{1-r} \]

\subsection*{construction}

The idea of the new proof is that a right triangle with angle $\theta$ (magenta dot) can be combined with scaled versions of itself to give a different right triangle with angle $2 \theta$, as shown in the figure.

\begin{center} \includegraphics [scale=0.4] {pythagoras17.png} \end{center}

All the smaller triangles are similar.  We will work out the lengths of these pieces in terms of the original triangle's sides.

Let the secant ($\sec \theta$) be $S = c/b$ and the tangent $T = a/b$.  Then the small triangles have sides:

\[ x = 2aS, \ \ \ \ \ \ p = 2a T \]
\[ d = pS = 2aST, \ \ \ \ \ \ v = pT = 2aT^2 \]
\[ y = vS = 2aST^2, \ \ \ \ \ \ q = vT = 2aT^3 \]
\[ e = qS = 2aST^3, \ \ \ \ \ \ w = qT = 2aT^4 \]
\[ z = wS = 2aST^4, \ \ \ \ \ \ r = wT = 2aT^5 \]

The last value to check is
\[ f = rS = 2aST^5 \]

Let us call the top side of the whole large right triangle $C$ and the bottom side $A$.  We have that
\[ A = x + y + z + \dots\]
\[ C = c + d + e + f \dots \]

Looking at the above results, A and C (minus the first term, $c$) are geometric series with the same ratio, $T^2$.

\[ x = 2aS, \ \ \ \ y = 2aST^2, \ \ \ \  z = 2aST^4 \]
\[ d = 2aST, \ \ \ \ e = 2aST^3, \ \ \ \  f = 2aST^5 \]

As we said, the sum of a geometric series with ratio $r$ and initial term $1$ is $1/(1-r)$, provided that $|r| < 1$.  Here $T = a/b$  If $b > a$ then $T > 1$ and then $1/T^2 < 1$, so the series converges.  If $a > b$ then just swap $a$ and $b$.  We deal with the case $a = b$ at the end.

The sum for initial term $k$ is 
\[ S = k \cdot \frac{1}{1-r} \]

This series has ratio $T^2$ so its sum is
\[A = 2aS \cdot \frac{1}{1-T^2} \]

Recalling that $S = c/b$ and $T = a/b$ so 
\[ aS = ac/b = cT \]
and then
\[ A = 2cT \cdot \frac{1}{1-T^2} \]

The other series is
\[ d + e + f + \dots = 2aST \cdot \frac{1}{1-T^2} \]

Using again the relation $aS = ac/b = cT$ we obtain 
 \[ d + e + f + \dots = \frac{2cT^2}{1 - T^2} \]

The whole of the top side $C$ is $c + d + e + f + \dots$
\[ C = c + \frac{2cT^2}{1 - T^2} \]
\[ = c \ (1 + \frac{2T^2}{1 - T^2} ) = c \cdot \frac{1 + T^2}{1 - T^2}  \]

We can finally form the ratio $A/C$, canceling the factor of $1 - T^2$.
\[ \frac{A}{C} = \frac{2cT}{c(1 + T^2)} \]
\[ = \frac{2a/b}{1 + a^2/b^2} \]
\[ = \frac{2ab}{a^2 + b^2} \]

The ratio $A/C$ is also the sine of the double angle $2 \theta$.

\subsection*{law of sines}

In any triangle, drop the altitude from vertex $C$ to the opposite side.
\begin{center} \includegraphics [scale=0.4] {triangle5.png} \end{center}

\[ \sin A = \frac{h}{b} \]
\[ \sin B = \frac{h}{a} \]
So
\[ b \sin A = a \sin B \]
The law of sines follows:
\[ \frac{b}{\sin B} = \frac{a}{\sin A} \]

Apply the law of sines to the isosceles (double) triangle with angle $2 \theta$ and sides $c$ and $2a$:

\[ \frac{\sin 2 \theta}{2a} = \frac{\sin (90-\theta)}{c} = \frac{\cos \theta}{c} = \frac{b}{c^2} \]
\[ \sin 2 \theta = \frac{2ab}{c^2} \]

Substituting the ratio of $A/C$ for the left-hand side:
\[ \frac{2ab}{a^2 + b^2} = \frac{2ab}{c^2} \]

The Pythagorean theorem immediately follows.

Finally, we must handle the case where $a = b$.  Then the small triangles are all isosceles as well.  So $\theta = 45^{\circ}$ and $2 \theta = 90^{\circ}$ and a square is formed with sides $c$.  

The ratio of opposing sides $C/A =  c/c = 1 = \sin 2 \theta$.  

The law of sines gives
\[ \frac{\sin 2 \theta}{2a} = \frac{\sin \theta}{c} \]
Since $\sin 2 \theta = 1$ and $\sin \theta = a/c$
\[ \frac{1}{2a} = \frac{a/c}{c} \]
\[ c^2 = 2a^2 \]
\[ = a^2 + b^2 \]

$\square$

\end{document}